{
 "cells": [
  {
   "cell_type": "markdown",
   "id": "b65fa415",
   "metadata": {},
   "source": [
    "# Introduction to Probability Generating Functions\n",
    "\n",
    "\n",
    "In this subject we will study probability generating functions.  We'll learn that they are very useful for understand branching processes.  A branching process is a type of random process where objects produce new objects.  These occur frequently in biological system where the objects might be cells or organisms, or infections, or any of a large number of biological things that replicate themselves.\n",
    "\n",
    "Before we get deep into the biology and applications of probability generating functions in biology, we'll start by learning about generating functions and then specifically about probability generating functions.\n",
    "\n"
   ]
  },
  {
   "cell_type": "markdown",
   "id": "1ab818ef",
   "metadata": {},
   "source": [
    "\n",
    "The reason for this is that the operations of adding, multiplying and more with Taylor Series turn out to be exactly the same as operations that occur when we are looking at how population sizes change in birth-death processes.\n",
    "\n",
    "Mathematicians give this a fancy name and say that these two mathematical systems are *isomorphic*.  In other words you will get the same answers no matter which of the mathematical systems you study.  Any results calculated in one system tells us about the corresponding results in the other system.\n",
    "\n",
    "Specifically given some sort of invasive biological process: \n",
    "    1. we can convert the process into the Taylor Series of one or multiple PGFs of $x$\n",
    "    2. We do some mathematical operations with the corresponding functions of $x$ to get a new PGF.\n",
    "    3. We can use the properties of the Taylor Series of the final answer to gain meaningful information about the original biological problem.\n",
    "\n",
    "\n",
    "Before we explore the correspondance between PGFs and birth-death processes, we introduce PGFs and show some of the manipulations that can be done with them.\n",
    "\n",
    "## Probability Generating Functions\n",
    "\n",
    "We start with two definitions:\n",
    "\n",
    "````{prf:definition} Generating Function\n",
    ":label: defGeneratingFunction\n",
    "\n",
    "Given a sequence of numbers $a_0$, $a_1$, $a_2$, \\ldots, the corresponding **generating function** is\n",
    "\n",
    "$$\n",
    "f(x) = \\sum_{n=0}^\\infty a_n x^n\n",
    "$$\n",
    "````\n",
    "Any polynomial is a generating function\n",
    "\n",
    "````{prf:example} $f(x)=1-x+x^2$\n",
    "The function $f(x)=1-x+x^2$ is a generating function for which $a_0=1$, $a_1=-1$, $a_2=1$, and $a_n=0$ for $n \\geq 3$.\n",
    "````\n",
    "\n",
    "````{prf:example} $f(x) = 1 + x + x^2 + \\cdots + x^k$.\n",
    "The function \n",
    "\n",
    "$$\n",
    "f_k(x) = 1 + x + x^2 + \\cdots + x^k\n",
    "$$ \n",
    "is an important PGF.  If we multiply $f(x)$ by $x-1$ and sum the values we get\n",
    "\n",
    "\\begin{align*}\n",
    "f_k(x)(1-x) &= -1 +x + x(-1+x) + x^2 (-1+x) + \\cdots + x^k(-1+x)\\\\\n",
    "          &= -1 + (x-x) + (x^2-x^2) \\cdots + (x^k-x^k) + x^{k+1}\\\\\n",
    "          &= -1 + x^{k+1}\n",
    "\\end{align*}\n",
    "So for $x\\neq 1$, we can rewrite $f_k(x)$ as $f_k(x)=(x^{k+1}-1)/(x-1)$, while for $x=1$ it is $f_k(1) = k+1$.  Thus\n",
    "\n",
    "$$\n",
    "f_k(x) = \n",
    "\\begin{cases} \\frac{x^{k+1}-1}{x-1} & x \\neq 1\\\\ k+1 & x=1\n",
    "\\end{cases}\n",
    "$$\n",
    "````\n",
    "\n",
    "More broadly, any function for which we can write out the Taylor Series can be thought of as a generating function.  The number of terms can be infinite.\n",
    "\n",
    "````{prf:example} $f(x)=e^{3x}$\n",
    "The function\n",
    "\n",
    "$$\n",
    "e^{3x} = 1 + 3x + \\frac{(3x)^2}{2} + \\frac{(3x)^3}{3!} + \\cdots \n",
    "$$\n",
    "is a generating function for the sequence $1, 3, 9/2, \\ldots, 3^n/n!, \\ldots$.\n",
    "````\n",
    "\n",
    "\n",
    "There are many useful applications of generating functions, some of which we'll explore momentarily, but first we define a special subtype that occurs when the sequence $a_0, a_1, \\ldots$ corresponds to a probability distribution on $0, 1, 2, \\ldots$. That is, $a_n$ gives the probability of the integer $n$. We usually use $p_n$ rather than $a_n$ to highlight the relation to probabilities.  By properties of probability distributions, we have $0 \\leq p_n \\leq 1$ for all $n$ and $\\sum_i p_n=1$  \n",
    "\n",
    "````{prf:definition} Probability Generating Function\n",
    ":label: def_PGF\n",
    "\n",
    "If\n",
    "\n",
    "$$ \n",
    "\\mu(x) = \\sum_n p_n x^n\n",
    "$$\n",
    "where $0 \\leq p_n$ and $\\sum_{n=0}^\\infty p_n = 1$, then $\\mu(x)$\n",
    "is a **Probability Generating Function**.\n",
    "````\n",
    "\n",
    "````{prf:example} $e^{x-1}$\n",
    "The function \n",
    "\n",
    "$$\n",
    "e^{\\lambda(x-1)} = \\sum_{n=0}^\\infty \\frac{\\lambda^n}{e^\\lambda n!} x^n\n",
    "$$\n",
    "is a PGF for any non-negative number $\\lambda$.\n",
    "````\n",
    "\n",
    "\n",
    "````\n",
    "... is a pgf if $f(1)=1$ and taylor series is made up of non-negative values.\n",
    "````"
   ]
  },
  {
   "cell_type": "markdown",
   "id": "72244a20",
   "metadata": {},
   "source": [
    "## Interesting examples\n",
    "\n",
    "````{prf:example} The Fibonacci Sequence\n",
    "\n",
    "Consider the Fibonacci numbers $F_k = F_{k-1} + F_{k-2}$ for $k \\geq 2$ and $F_0 =0$,  $F_1 = 1$.\n",
    "\n",
    "Let\n",
    "\n",
    "$$\n",
    "f(x) = \\sum_k F_k x^k\n",
    "$$\n",
    "Using the recurrence\n",
    "\n",
    "\\begin{align*}\n",
    "f(x) &= F_0 + F_1 x + \\sum_{k=2}^\\infty F_k x^k\\\\\n",
    "&= x+  \\sum_{k=2}^\\infty (F_{k-1}+F_{k-2})x^k\\\\\n",
    "&= x + \\sum_{k=2}^\\infty F_{k-1}x^{k} + F_{k-2}x^{k}\\\\\n",
    "&= x + \\sum_{k=1}^\\infty F_k x^{k+1} + \\sum_{k=0}^\\infty F_k x^{k+2}\\\\\n",
    "&= x + x (f(x) - F_0) + x^2f(x)\\\\\n",
    "&= x + xf(x)  + x^2 f(x)\\\\\n",
    "(1-x-x^2)f(x) &= x\n",
    "\\end{align*}\n",
    "\n",
    "So\n",
    "\n",
    "$$\n",
    "f(x) = \\frac{-x}{x^2+x-1}\n",
    "$$\n",
    "\n",
    "We want to find an explicit formula for the coefficients of the expansion of $f(x)$.  We know that $A/(1-\\alpha x) = A(1 + \\alpha x + (\\alpha x)^2 + \\cdots)$.  \n",
    "\n",
    "So we'll try to write $f(x)$ as the sum of two such functions.  You've likely done something like this before when using partial fractions to do an integral.  We'll revisit that method.  Don't worry if you don't recall it, we'll walk through it.  \n",
    "\n",
    "First we factor the denominator \n",
    "\n",
    "\\begin{align*}\n",
    "x^2 + x - 1 &= \\left( x - \\frac{-1 + \\sqrt{1+4}}{2}\\right) \\left(x - \\frac{-1 - \\sqrt{1+4}}{2}\\right)\\\\\n",
    "&= (x+1-\\phi)(x+\\phi)\n",
    "\\end{align*}\n",
    "where $\\phi = (1+\\sqrt{5})/2$ is the *golden ratio*.  One property of $\\phi$ is that $1-\\phi=-1/\\phi$.  We expand $f(x)$ using partial fractions\n",
    "\n",
    "\\begin{align*}\n",
    "\\frac{-x}{x^2+x-1} &= \\frac{A}{x-1/\\phi} + \\frac{B}{x+\\phi}\\\\\n",
    "-x &= A(x+\\phi) + B(x-1/\\phi)\n",
    "\\end{align*}\n",
    "After enough fiddling, $A = -1/\\phi\\sqrt{5}$ and $B = -\\phi/\\sqrt{5}$.  We put this together and then convert it to a form resembling the formula for a geometric series.\n",
    "\n",
    "\\begin{align*}\n",
    "f(x) &=  \\frac{-1/\\sqrt{5}\\phi}{ x - 1/\\phi} + \\frac{-\\phi/\\sqrt{5}}{x+\\phi}\\\\\n",
    "&= \\frac{1}{\\sqrt{5}} \\left(\\frac{1}{1-\\phi x} - \\frac{1}{1- (-1/\\phi) x} \\right)\\\\\n",
    "&= \\frac{1}{\\sqrt{5}} \\left( \\sum_{n=0}^\\infty (\\phi x)^n - \\sum_{n=0}^\\infty (-x/\\phi)^n\\right)\\\\\n",
    "&= \\frac{1}{\\sqrt{5}} \\sum_{n=0}^\\infty \\left(\\phi^n -(-1/\\phi)^n\\right)x^n\n",
    "\\end{align*}\n",
    "\n",
    "So we conclude that $F_n = \\frac{\\phi^n - (-1/\\phi)^n}{\\sqrt{5}}$.\n",
    "````\n",
    "\n"
   ]
  },
  {
   "cell_type": "markdown",
   "id": "e2818da3",
   "metadata": {},
   "source": [
    "\n",
    "````{prf:example} $\\sum_{k=0}^n k \\binom{n}{k}$\n",
    "Consider the sum $\\sum{k=0}^n k \\binom{n}{k}$.  We start with a related generating function\n",
    "\n",
    "$$\n",
    "f(x) = \\sum_{k=0}^n \\binom{n}{k} x^k\n",
    "$$\n",
    "Then we perform a trick which multiplies each term in the sum by $k$ (which is different for each term).  The way we do this is by differentiating $f(x)$.  That multiplies each term by $k$, but it also reduces the power of $x$ by $1$.  So after we differentiate, we multiply by $x$.  So we look at\n",
    "\n",
    "$$\n",
    "x f'(x) = x \\sum_{k=0}^n \\binom{n}{k} k x^{k-1} = \\sum_{k=0}^n \\binom{n}{k} x^k\n",
    "$$\n",
    "The value of $xf'(x)$ at $x=1$ will be this sum.  To get it, we just note that $f(x) = \\sum_{k=0}^n \\binom{n}{k} x^k = (1+x)^n$.  So $x f'(x) = xn(1+x)^{n-1}$.  Thus setting $x=1$,\n",
    "\n",
    "$$\n",
    "n2^{n-1} = \\sum_{k=0}^n k \\binom{n}{k} \n",
    "$$\n",
    "\n",
    "````\n",
    "\n",
    "````{prf:example} Expected value of a geometric distribution\n",
    "\n",
    "$p$\n",
    "\n",
    "$p_1 = p$,\n",
    "\n",
    "$p(X\\geq {k-1}) = (1-p)^{k-1}$\n",
    "\n",
    "$p_k = p(1-p)^{k-1}$\n",
    "\n",
    "Find the expected value of a geometric distribution.\n",
    "\n",
    "$$\n",
    "\\sum_k k p (1-p)^{k-1} = p \\sum_k k (1-p)^{k-1} = p \\sum_{k=1}^\\infty \\left. \\frac{d}{dx} x^k \\right|_{x=(1-p)} = p \\left.\\frac{d}{dx} \\frac{x}{1-x}\\right|_{x=(1-p)} = p \\left.\\frac{1-x - x(-1)}{(1-x)^2}\\right|_{x=1-p} = p \\frac{1}{p^2} = 1/p\n",
    "$$\n",
    "\n",
    "````\n",
    "\n",
    "The \"multiply by k\" trick used above will be used several times in this course."
   ]
  },
  {
   "cell_type": "markdown",
   "id": "40855bf5",
   "metadata": {},
   "source": [
    "### Optional example, for those who are really keen\n",
    "\n",
    "Now we consider a final example showing how ordinary generating functions can be used to derive some identities.   After this we will mostly set these aside and focus specifically on probability generating functions.\n",
    "\n",
    "````{prf:example} $\\sum_{n=0}^k n^2$\n",
    "Consider the sum $\\sum_{n=0}^k n^2$.  You may have asked to prove a formula for this using induction, but it is unlikely you were expected to come up with the formula.  Standard approaches for this problem are generally messy.\n",
    "\n",
    "Let us consider the function\n",
    "\n",
    "$$\n",
    "f_k(x) = \\sum_{n=0}^k 1 x^n = \\begin{cases} \\frac{1-x^{k+1}}{1-x} & x \\neq 1\\\\\n",
    "k+1 & x=1\n",
    "\\end{cases}\n",
    "$$\n",
    "It is possible to use the multiply by $n$ trick twice on this to find\n",
    "\n",
    "$$\n",
    "\\left.\\left ( x \\frac{d}{dx} \\left( x \\frac{d}{dx} f_k(x)\\right)\\right)\\right|_{x=1}\n",
    "$$\n",
    "However, solving at this point requires some applications of L'Hopital's rule and can get difficult.\n",
    "\n",
    "Instead we take a different approach.  Ultimately we are going to find a generating function of the form \n",
    "\n",
    "$$\n",
    "g(x) = 0^2 x^0 + 1^2 x^1 + (1^2+2^2) x^2 + \\cdots = \\sum_{n=0}^\\infty \\left(\\sum_{j=0}^n j^2 \\right) x^n\n",
    "$$\n",
    "\n",
    "We start with the infinite geometric series\n",
    "\n",
    "$$\n",
    "f(x) = 1 + x + x^2 + \\cdots = \\sum_{n=0}^\\infty x^n\n",
    "$$\n",
    "This series becomes\n",
    "\n",
    "$$\n",
    "f(x) = \\frac{1}{1-x}\n",
    "$$\n",
    "and it is guaranteed to converge for any $|x|<1$. \n",
    "\n",
    "Using the \"multiply by $n$ trick\" twice now and changing the summation index to $j$ rather than $n$ gives\n",
    "\n",
    "$$\n",
    "x(xf'(x))' = \\sum_{j=0}^\\infty j^2 x^j\n",
    "$$\n",
    "\n",
    "Now we consider the product\n",
    "\n",
    "$$\n",
    "g(x)=\\left(\\sum_{i=0}^\\infty x^i\\right) \\left(\\sum_{j=0}^\\infty j^2 x^j\\right) = \\left( 1x^0 + 1x^1 + 1x^2 + \\cdots\\right) \\left( 0x^0 + 1^2x^1 + 2^2 x^2 + 3^2 x^3 + \\cdots\\right)\n",
    "$$\n",
    "If we consider the coefficient of $x^n$, we take each $i$ and $j$ that sum to $n$, multiply the coefficients, and sum the result for each pair.  The coefficient of $x^n$ is thus $1\\cdot 0^2 + 1\\cdot 1^2 + \\cdots + 1\\cdot n^2$.  That is\n",
    "\n",
    "$$\n",
    "g(x)=\\left(\\sum_{i=0}^\\infty x^i\\right) \\left(\\sum_{j=0}^\\infty j^2 x^j\\right) = \\sum_{n=0}^\\infty \\left(\\sum_{j=0}^n j^2 \\right) x^n\n",
    "$$\n",
    "This is the generating function whose entries are the sums we want.\n",
    "\n",
    "Analyzing the generating functions we multiplied together, we have\n",
    "\n",
    "\\begin{align*}\n",
    "g(x) &= \\frac{1}{1-x} x(xf'(x))'\\\\\n",
    "   &= \\frac{x}{1-x} [f'(x) + x f''(x)]\\\\\n",
    "   &= \\frac{x}{1-x} \\left[ \\frac{d}{dx} (1-x)^{-1}+ x \\frac{d^2}{(dx)^2} (1-x)^{-1}\\right]\\\\\n",
    "   &= \\frac{x}{1-x} \\left [ -1(1-x)^{-2}(-1) + (-2)(1-x)^{-3}(-1)\\right]\\\\\n",
    "   &= x\\left((1-x)^{-3} + 2(1-x)^{-4}\\right)\n",
    "\\end{align*}\n",
    "A generalization of the binomial theorem states that \n",
    "\n",
    "$$\n",
    "(a+b)^{r} = a^r + \\frac{r}{1} a^{r-1}b + \\frac{r(r-1)}{2!} a^{r-2} b^2 + \\frac{r(r-1)(r-2)}{3!}  a^{r-3}b^3 + \\cdots \n",
    "$$\n",
    "In the case where $r=-s$ is negative, this can be written\n",
    "\n",
    "\\begin{align*}\n",
    "(a+b)^{-s} &= a^{-s} + \\frac{-s}{1} a^{-s-1}b + \\frac{(-s)(-s-1)}{2!} a^{-s-2} b^2 + \\frac{(-s)(-s-1)(-s-2)}{3!}  a^{-s-3}b^3 + \\cdots \\\\\n",
    "&= a^{-s} + (-1)^1 \\binom{s}{1} a^{-s-1}b + (-1)^2\\binom{s+1}{2} a^{-s-2}b^2 + (-1)^3\\binom{s+2}{3} a^{-s-3}b^3 + \\cdots \\\\\n",
    "&= \\sum_{j=0}^\\infty (-1)^j \\binom{s+j-1}{j}a^{-s-j}b^j \n",
    "\\end{align*}\n",
    "In our case $a = 1$, $b=-x$.  So for us\n",
    "\n",
    "$$\n",
    "(1-x)^{-s} = \\sum_{j=0}^\\infty \\binom{s+j-1}{j} x^j = \\sum_{j=0}^\\infty \\binom{s+j-1}{s-1} x^j\n",
    "$$\n",
    "So since $s=3$ or $s=4$:\n",
    "\n",
    "\\begin{align*}\n",
    "g(x) =& x \\left ( \\sum_{j=0}^\\infty \\binom{3+j-1}{2} x^j + \\sum_{j=0}^\\infty \\binom{4+j-1}{3} x^j\\right)\\\\\n",
    "&= x \\left( \\sum_{j=0}^\\infty \\left[\\binom{j+2}{2} + \\binom{j+3}{3} \\right] x^j \\right)\\\\\n",
    "&= \\sum_{n=1}^\\infty \\left[\\binom{n+1}{2} + \\binom{n+2}{3}\\right]x^n\\\\\n",
    "\\end{align*}\n",
    "So we predict that the sum $1^2+2^2+3^2+\\cdots + n^2$ must be the coefficient of $x^n$ which is \n",
    "\n",
    "$$\n",
    "\\binom{n+1}{2} + \\binom{n+2}{3} = \\sum_{j=0}^n j^2\n",
    "$$\n",
    "\n",
    "reference: https://math.stackexchange.com/a/1802085/201006\n",
    "````\n",
    "In this example, we used the fact that if we multiply a generating function $f(x)$ by $1+x+x^2+\\cdots = 1/(1-x)$, then we get a new generating function whose coefficients of $x^n$ is equal to the sum of the coefficients of powers of $x$ up to $x^n$ in $f(x)$."
   ]
  },
  {
   "cell_type": "markdown",
   "id": "b0da1147",
   "metadata": {},
   "source": []
  },
  {
   "cell_type": "markdown",
   "id": "9d27e4b4",
   "metadata": {},
   "source": []
  },
  {
   "cell_type": "markdown",
   "id": "2b412df2",
   "metadata": {},
   "source": [
    "## Properties of generating functions and applications\n",
    "\n",
    "$f(1)$ is sum\n",
    "\n",
    "$n\\frac{d}{dx} f(x)$ is generating function $\\sum_n n a_n x^{n}$\n",
    "\n",
    "To get the sum\n",
    "$1 + 2 + 3 + \\cdots + k$\n",
    "we start with \n",
    "\n",
    "\\begin{align*}\n",
    "f_k(x) &= (x+x^2+\\cdots + x^k)\\\\\n",
    "&= \n",
    "\\begin{cases} \\frac{1-x^{k+1}}{1-x} & x \\neq 1\\\\ k+1 & x=1\n",
    "\\end{cases}\n",
    "\\end{align*}\n",
    "Then \n",
    "\n",
    "$$\n",
    "f_k'(x) = 1 + 2x + 3x^2 + \\cdots + k x^{k-1}\n",
    "$$\n",
    "So\n",
    "\n",
    "$$\n",
    "f_k'(1) = 1 + 2 + \\cdots + k\n",
    "$$\n",
    "\n",
    "Since $f_k(x) = \\frac{x^{k+1}-1}{x-1}$ for $x\\neq 1$, we have\n",
    "\n",
    "$$f_k'(x) = \\frac{(x-1)(k+1)x^k - (x^{k+1}-1)1}{(x-1)^2}\n",
    "$$\n",
    "We could use two applications of L'Hopital's rule to find $f_k'(1)$, but a more elegant approach starts by substituting $u = x-1$ or $x = 1+u$ where we assume $u$ is small into this expression.\n",
    "\\begin{align*}\n",
    "f_k'(x) &= \\frac{u(k+1)(1+u)^k - ((1+u)^{k+1}-1)}{u^2}\\\\\n",
    "&= \\frac{(k+1)(u + ku^2+ \\mathcal{O}(u^3)) - ((k+1)u + \\frac{(k+1)(k)}{2}u^2 + \\mathcal{O}(u^3))}{u^2}\\\\\n",
    "&=(k+1)(k) - \\frac{(k+1)(k)}{2} + \\mathcal{O}(u)\\\\\n",
    "&= \\frac{(k+1)(k)}{2} + \\mathcal{O}(u)\n",
    "\\end{align*}\n",
    "\n",
    "\n",
    "\n",
    "PGFs\n",
    "\n",
    "$\\mu(1) = 1$\n",
    "\n",
    "Expected value of $n$ is $\\left.\\frac{d}{dx}\\mu(x)\\right|_{x=1}$.\n",
    "\n",
    "Expected value of $n^2$ is $\\left. \\frac{d}{dx} x \\frac{d}{dx} \\mu(x) \\right |_{x=1}$\n"
   ]
  },
  {
   "cell_type": "markdown",
   "id": "5a3b1d90",
   "metadata": {},
   "source": [
    "## Applications of Generating Functions\n",
    "\n",
    "\n",
    "One common application of generating functions is in calculating sums of terms that involve the index $n$.  For example\n",
    "\n",
    "\n",
    "\n",
    "Specifically to PGFs, we can use them to calculate expected values.\n"
   ]
  }
 ],
 "metadata": {
  "language_info": {
   "name": "python"
  }
 },
 "nbformat": 4,
 "nbformat_minor": 5
}
