{
 "cells": [
  {
   "cell_type": "markdown",
   "id": "5cb1f72f",
   "metadata": {},
   "source": [
    "# Generating Function Examples\n",
    "\n"
   ]
  },
  {
   "cell_type": "markdown",
   "id": "35cd6460",
   "metadata": {},
   "source": [
    "```{prf:example} Geometric Sequences\n",
    "\n",
    "Consider the generating function for the sequence $1, 1, 1, 1, \\ldots$.  It is given by $f(x) = 1 + x + x^2 + \\cdots$\n",
    "\n",
    "$$\n",
    "f(x) = 1 + x + x^2 + \\cdots\n",
    "$$\n",
    "If you remember the formula for a geometric series, this can be written in compact form:\n",
    "\n",
    "$$\n",
    "f(x) = \\frac{1}{1-x} = \\frac{-1}{x-1}\n",
    "$$\n",
    "This converges for $|x|<1$.\n",
    "```\n",
    "\n",
    "```{prf:remark}\n",
    "If you don't remember the formula for the geometric series, define $f_N(x) = 1 + x + x^2 + \\cdots + x^N$.  Multiply it by $1-x$:\n",
    "\n",
    "\\begin{align*}\n",
    "f_N(x)(1-x) &= f_N(x) - x f_N(x)\\\\\n",
    "&= (1 + x + x^2 +\\cdots +x^N ) - (x + x^2 + \\cdots + x_N)\\\\\n",
    "&= 1-x^N\n",
    "\\end{align*}\n",
    "So $f_N(x) = (1-x^N)/(1-x)$.  Assuming $|x|<1$, then taking $N \\to \\infty$ gives $f(x) = \\lim_N \\to \\infty f_N(x) = 1/(1-x)$\n",
    "```\n",
    "\n",
    "In the self-test below, you will show that $f(x) = Ab/(b-x) = -Ab/(x-b)$ is the generating function for the sequence $A, A/b, A/b^2, \\ldots$.\n",
    "\n"
   ]
  },
  {
   "cell_type": "markdown",
   "id": "f347df15",
   "metadata": {},
   "source": [
    "```{prf:example} The Fibonacci sequence\n",
    ":label: ex-fibonacci_fxn\n",
    "\n",
    "Consider the Fibonacci sequence defined by $F_0=0$, $F_1 = 1$ and $F_{n} = F_{n-1}+ F_{n-2}$ for $n \\geq 2$.  Given this sequence of numbers, we can define the generating function of the Fibonacci sequence:\n",
    "\n",
    "\\begin{align*}\n",
    "f(x) &= F_0 + F_1 x + F_2 x^2 + F_3 x^3 + F_4x^4+F_5x^5+F_6x^6+\\cdots \\\\\n",
    "&= 0 + x + 1x^2 + 2x^3 + 3 x^4 +5x^5 + 8x^6+\\cdots\n",
    "\\end{align*}\n",
    "\n",
    "Let's try to write this as a compact expression.  We need to use $F_n = F_{n-1}+ F_{n-2}$ to figure out what $f(x)$ is.  We start with the definition of a generating function, and then we use properties of the Fibonacci sequence.\n",
    "\n",
    "\\begin{align*}\n",
    "f(x) &= F_0 + F_1 x + F_2 x^2 + F_3 x^3 + \\ldots \\\\\n",
    "&= F_0 +  F_1 x + \\sum_{n=2}^\\infty F_nx^n\\\\\n",
    "&= F_0 + F_1 x + \\sum_{n=2}^\\infty (F_{n-1} + F_{n-2})x^n\\\\\n",
    "&= F_0 + F_1 x + \\sum_{n=2}^\\infty F_{n-2}x^n + \\sum_{n=2}^\\infty F_{n-1}x^n\\\\\n",
    "&= F_0 + F_1 x + x^2 \\sum_{n=2}^\\infty F_{n-2}x^{n-2} + x \\sum_{n=2}^\\infty F_{n-1} x^{n-1}\\\\\n",
    "&= F_0 + F_1 x + x^2 (F_0 + F_1x + F_2 x^2+\\cdots) + x (F_1x + F_2 x^2 + \\cdots)\\\\\n",
    "&= F_0 + F_1x + x^2f(x) + x (f(x)-F_0)\\\\\n",
    "&= x + (x+x^2)f(x)\n",
    "\\end{align*}\n",
    "using $F_0=0$ and $F_1=1$ for the last step, and the definition of $f(x)$ for the next to last step.\n",
    "\n",
    "Moving the terms with $f(x)$ onto the left hand side:\n",
    "\n",
    "\\begin{align*}\n",
    "f(x) ( 1- x - x^2) &= x\\\\\n",
    "\\Rightarrow f(x) &= \\frac{ x}{1-x-x^2}\n",
    "\\end{align*}\n",
    "```\n",
    "\n"
   ]
  },
  {
   "cell_type": "markdown",
   "id": "6e847b2a",
   "metadata": {},
   "source": [
    "## Probability Generating Functions\n",
    "\n",
    "We now look specifically at a few probability generating functions."
   ]
  },
  {
   "cell_type": "markdown",
   "id": "95b1ff09",
   "metadata": {},
   "source": [
    "```{prf:example} Flipping a fair coin\n",
    "Consider a fair coin.  We will set $n$ to be the number of heads from a single flip.  Then $p_0 =1/2$ and $p_1 = 1/2$ and $p_n = 0$ for $n\\geq 2$.\n",
    "\n",
    "Because this is a probabiity distribution for $0,1$, the resulting generating function is a **probabiliy generating function (PGF)**:\n",
    "\n",
    "$$\n",
    "f(x) = \\frac{1+x}{2}\n",
    "$$\n",
    "```"
   ]
  },
  {
   "cell_type": "markdown",
   "id": "4e11bd68",
   "metadata": {},
   "source": [
    "```{prf:example} Flipping a weighted coin\n",
    "Now consider a coin with probaibility $p_H$ of heads and $1-p_H$ of tails.  Again, we count the number of heads, so $p_0=1-p_H$ and $p_1 = p_H$\n",
    "\n",
    "Then the PGF is\n",
    "\n",
    "$$\n",
    "f(x) = (1-p_H) + p_H x\n",
    "$$\n",
    "```"
   ]
  },
  {
   "cell_type": "markdown",
   "id": "4ee797ab",
   "metadata": {},
   "source": [
    "```{prf:example} Multiple flips of a weighted coin\n",
    "\n",
    "Consider now the result of $n$ flips of a weighted coin.  The probability of $k$ heads is $\\binom{n}{k} p_H^k (1-p_H)^{n-k}$ (this is because there are $\\binom{n}{k}$ sequences that give $k$ heads and $n-k$ non-heads.  Each of those sequences occurs with probability $p_H^k (1-p_H)^{n-k}$).  \n",
    "\n",
    "Then the PGF is\n",
    "\n",
    "\\begin{align*}\n",
    "f(x) &= \\sum_{k=0}^n \\binom{n}{k} (1-p_H)^{n-k}p_H^k x^k\\\\\n",
    "&= (1-p_H)^n(p_Hx)^0 + n (1-p_H)^{n-1}(p_Hx) + \\frac{n(n-1)}{2} (1-p_H)^{n-2}(p_Hx)^{2} + \\cdots + \\frac{n!}{k!(n-k)!} (1-p_H)^{n-k}(p_Hx)^k + \\cdots + (1-p_H)^0(p_Hx)^n\\\\\n",
    "&= (1-p_H + p_Hx)^n\n",
    "\\end{align*}\n",
    "```\n",
    "\n",
    "```{prf:remark}\n",
    "\n",
    "Notice that the PGF for multiple flips is the PGF for a single flip raised to the $n$th power.  We will learn later why this happens.\n",
    "```\n"
   ]
  },
  {
   "cell_type": "markdown",
   "id": "14286f9c",
   "metadata": {},
   "source": [
    "\n",
    "```{prf:example} 6-sided dice\n",
    "\n",
    "Consider the probabilty of rolling a $k$ with a typical 6-sided die, for which $p_k = 1/6$ for $k=1, 2, \\ldots, 6$.\n",
    "\n",
    "The PGF is:\n",
    "\n",
    "\\begin{align*}\n",
    "f(x) &= \\frac{1}{6}x  + \\frac{1}{6}x^2  + \\ldots + \\frac{1}{6} x^6\\\\\n",
    "&= \\frac{1}{6} (x + x^2 + x^3 + x^4 + x^5 + x^6)\n",
    "\\end{align*}\n",
    "```"
   ]
  },
  {
   "cell_type": "markdown",
   "id": "290b2b99",
   "metadata": {},
   "source": [
    "## Self-test\n",
    "\n",
    "1. Consider the sequence $A, A/b, A/b^2, \\ldots$.\n",
    "   1.  Write down the generating function of this sequence in expanded form.\n",
    "   2.  Use the formula for the geometric series to find $f(x)$.\n",
    "   3.  For what values of $x$ does the series converge?\n",
    "\n",
    "2. (this extends the results of the previous question) Consider the function $g(x) = \\frac{5-4x}{x^2-3x+2}$.  \n",
    "   1.  Show that $g(x)=\\frac{1}{1-x} + \\frac{3}{2-x} = \\frac{1}{1-x} + \\frac{\\frac{3}{2} 2}{2-x}$ (later we will use partial fractions to break $g$ up into two terms like this, but for this question, start from this expansion and verify that you can combine the terms to get the original $g(x)$).\n",
    "   2.  Expand the two fractions above into power series using Question 1.\n",
    "   3.  Use this to write down the power series of $g(x)$.  Find a formula for the $n$-th coefficient of the generating function.\n",
    "   4.  Using   $g(x) = \\frac{5-4x}{x^2-3x+2}$, find $g(0)$ and $g'(0)$.     Verify that the generating function you found is equal to $g(0) + g'(0)x + \\cdots$.\n",
    "\n",
    "\n"
   ]
  }
 ],
 "metadata": {
  "language_info": {
   "name": "python"
  }
 },
 "nbformat": 4,
 "nbformat_minor": 5
}
