{
 "cells": [
  {
   "cell_type": "markdown",
   "id": "1e5b88fc",
   "metadata": {},
   "source": [
    "# Partial Fractions\n",
    "\n",
    "Given a function $f(x)$, there are multiple ways that we can extract the coefficients of its Taylor Series.  When a function $f(x)$ is written as a rational function (that is, the ratio of two polynomials), f(x) = p(x)/q(x)$, one way is through partial fractions.\n",
    " \n",
    "\n",
    "We will look at how to write $f(x)=p(x)/q(x)$ in partial fractions assuming that $f(x)$ satisfies the following criterion:\n",
    "```{prf:criterion}\n",
    ":label: crit-rational\n",
    "- the fraction is reduced ($p$ and $q$ share no common non-constant factors)\n",
    "- the denominator $q(x)$ is a degree $k$ polynomial, \n",
    "- the numerator $p(x)$ has degree less than $k$, and \n",
    "- $q(x)=0$ has $k$ different, nonzero roots (the roots do not need to be real).  \n",
    "```\n",
    "\n",
    "If any roots of $q(x)=0$ are repeated, some more nuanced techniques will be needed than what we look at here.  If $x=0$ is a root, then the original function cannot be written as a generating function: $f(x) \\neq c_0 +c_1 x + \\cdots$.\n",
    "\n",
    "## The method of partial fractions\n",
    "We will show the partial fractions technique for an arbitrary function $f(x)$ that satisfies the assumptions above.  Then we will work through an example. \n",
    "\n",
    "Consider the function $f(x) = p(x)/q(x)$ where $p$ and $q$ are polynomials and $q(0) \\neq 0$.  We scale $p$ and $q$ so that the leading term of $q$ is $x^k$. Then $q(x)$ is a product of distinct linear terms:\n",
    "\n",
    "$$q(x)=\\prod_{i=1}^k (x-b_i)$$\n",
    "\n",
    "We can write\n",
    "\n",
    "$$\n",
    "f(x) = \\frac{p(x)}{(x-b_1)(x-b_2)(x-b_3)(x-b_4)\\cdots(x-b_k)} = \\frac{-A_1b_1}{(x-b_1)} + \\frac{-A_2 b_2}{x-b_2}  + \\cdots + \\frac{-A_kb_k}{x-b_k}\n",
    "$$\n",
    "\n",
    "```{prf:remark}\n",
    "Often you will see Partial Fractions given without the $b_i$ in the numerator, using \n",
    "\n",
    "$$\n",
    "\\frac{p(x)}{(x-b_1)(x-b_2)(x-b_3)(x-b_4)\\cdots(x-b_k)} = \\frac{C_1}{(x-b_1)} + \\frac{C_2}{x-b_2}  + \\cdots + \\frac{C_k}{x-b_k}\n",
    "$$\n",
    "\n",
    "It is fine to do this, but eventually you'll have to do an extra step to write $C_k = -A_k b_k$, so I find it easier to already start with $A_i$ being the term I want.  Feel free to approach this however you prefer\n",
    "```\n",
    "\n",
    "If we multiply by the denominator $q(x)$, we have\n",
    "\n",
    "\\begin{align*}\n",
    "p(x) &= -A_1 b_1\\prod_{j\\neq 1} (x-b_j) - A_2 b_2 \\prod_{j \\neq 2} (x-b_j)  - \\cdots - A_k b_k \\prod_{j \\neq k} (x-b_j)\\\\\n",
    "&= \\sum_{i=1}^k \\left(-A_i b_i\\prod_{j \\neq i} (x-b_j)\\right)\n",
    "\\end{align*}\n",
    "There are many techniques that can be used to solve this.  However, for the case that we are considering, the easiest is to set $x = b_1$, then $x=b_2$, etc.  Each time, most of the products on the right hand side are zero.  We get the equations:\n",
    "\n",
    "\\begin{align*}\n",
    "p(b_1) &= -A_1 b_1 \\prod_{j\\neq 1} (b_1-b_j)\\\\\n",
    "p(b_2) &= -A_2 b_2 \\prod_{j \\neq 2} (b_2-b_j)\\\\\n",
    "\\vdots &\\vdots \\qquad \\qquad \\vdots\\\\\n",
    "p(b_k) &= -A_k b_k \\prod_{j \\neq k} (b_k-b_j)\n",
    "\\end{align*}\n",
    "\n",
    "So we can immediately find \n",
    "\n",
    "$$\n",
    "A_i = -\\frac{p(b_i)}{ b_i \\prod_{j \\neq i} (x-b_j)}\n",
    "$$\n",
    "and once we have $A_i$, we have found\n",
    "\n",
    "\\begin{align*}\n",
    "f(x) &= \\sum_{i=1}^k \\frac{-A_i b_i}{x-b_i}\\\\\n",
    "&= \\sum_{i=1}^k \\left(A_i + \\frac{A_i}{b_i}x + \\frac{A_i}{b_i^2} x^2 + \\cdots\\right)\\\\\n",
    "&= (\\sum A_i) + (\\sum \\frac{A_i}{b_i}) x + (\\sum \\frac{A_i}{b_i^2}) x^2 + \\cdots\n",
    "\\end{align*}\n",
    "\n",
    "\n",
    "```{prf:remark}\n",
    "In fact, we can simplify this one further step by noting that \n",
    "\n",
    "$$\n",
    "q'(x) = \\sum_{i=1}^k \\prod_{j \\neq i} (x-b_j)\n",
    "$$\n",
    "and setting $x = b_i$ for some $i$ will yield zero for most terms\n",
    "\n",
    "$$\n",
    "q'(b_i) = \\prod_{j \\neq i} (b_i-b_j)\n",
    "$$\n",
    "So\n",
    "\n",
    "$$\n",
    "A_i = -\\frac{p(b_i)}{b_i q'(b_i)}\n",
    "$$\n",
    "```\n"
   ]
  },
  {
   "cell_type": "markdown",
   "id": "29570273",
   "metadata": {},
   "source": [
    "\n",
    "## Example: A formula for the Fibonacci numbers\n",
    "\n",
    "We have seen the the Fibonacci sequence $0, 1, 1, 2, 3, 5, \\ldots$ has generating function\n",
    "\n",
    "$$\n",
    "f(x) = \\frac{x}{1-x-x^2}\n",
    "$$\n",
    "\n",
    "We will apply the method above.  First, we rewrite\n",
    "\n",
    "$$\n",
    "f(x) = \\frac{-x}{x^2 + x -1}\n",
    "$$\n",
    "We find the roots of $x^2+x-1$ by using the quadratic formula\n",
    "$\\frac{-1 \\pm \\sqrt{1+4}}{2} = \\frac{-1 \\pm \\sqrt{5}}{2}$.  We will use $b_1 = -(1+\\sqrt{5})/2$.  This is the negative of the golden ratio $\\phi = \\frac{1+\\sqrt{5}}{2}$.  The other root is $b_2=(-1+\\sqrt{5})/2 $.  It will be simpler at first to just use $b_1$ and $b_2$ in the calculations:\n",
    "\n",
    "\\begin{align*}\n",
    "\\frac{-x}{x^2 + x -1} &= \\frac{-A_1b_1}{x-b_1} + \\frac{-A_2b_2}{x-b_2}\\\\\n",
    "-x &= -A_1 b_1(x-b_2) - A_2 b_2(x-b_1)\n",
    "\\end{align*}\n",
    "Setting $x=b_1$ and $x=b_2$, we find\n",
    "\n",
    "\\begin{align*}\n",
    "1 &= A_1(b_1-b_2)\\\\\n",
    "1 &= A_2(b_2-b_1) \\\\\n",
    "\\quad&\\\\\n",
    "\\Rightarrow  A_1 &= 1/(b_1-b_2)\\\\\n",
    " A_2 &= 1/(b_2-b_1) = - A_1 \n",
    "\\end{align*}\n",
    "\n",
    "Expanding out, we have\n",
    "\n",
    "\\begin{align*}\n",
    "f(x) &= \\frac{-A_1b_1}{x-b_1} + \\frac{-A_2b_2}{x-b_2}\\\\\n",
    "&= A_1 \\sum_{n=0}^\\infty \\frac{1}{b_1^n}x^n + A_2 \\sum _{n=0}^\\infty\\frac{1}{b_2^n} x^n\\\\\n",
    "&= A_1 \\sum_{n=0}^\\infty \\left(\\frac{1}{b_1^n} - \\frac{1}{b_2^n}\\right)x^n\n",
    "\\end{align*}\n",
    "We now write $b_1 = -\\phi$.  By checking, we can see that $b_1b_2 = -1$, so $b_2 = 1/\\phi$.  We can also see that $b_1-b_2 = -\\sqrt{5}$, so $A_1 = -1/\\sqrt{5}$.  Using all of these simplifications, we have\n",
    "\n",
    "\\begin{align*}\n",
    "f(x) &= -\\frac{1}{\\sqrt{5}} \\sum_{n=0}^\\infty \\left( \\frac{1}{(-\\phi)^n} - (\\phi)^n\\right)x^n\\\\\n",
    "&= \\frac{1}{\\sqrt{5}} \\sum_{n=0}^\\infty \\left( \\phi^n - \\frac{1}{(-\\phi)^n}\\right)x^n\n",
    "\\end{align*}\n",
    "Since \n",
    "\n",
    "$f(x) = F_0 + F_1 x + \\cdots$, we conclude that\n",
    "\n",
    "\n",
    "$$\n",
    "F_n = \\frac{\\phi^n - (-1/\\phi)^n}{\\sqrt{5}}\n",
    "$$\n",
    "where $\\phi = \\frac{1+\\sqrt{5}}{2}$ and $-1/\\phi = \\frac{ 1-\\sqrt{5}}{2}$."
   ]
  },
  {
   "cell_type": "markdown",
   "id": "6a2b8615",
   "metadata": {},
   "source": [
    "## Self-test\n",
    "\n",
    "1. Which of the following functions satisfy {prf:ref}`crit-rational`?  For each that does, find $p(x)$ and $q(x)$.\n",
    "   1. $f(x) = \\frac{1-x}{2(x^2+3x+2)}$\n",
    "   2. $f(x) = \\frac{1-x}{2x^2+3x}$\n",
    "   3. $f(x) = \\frac{-x}{2x^2-x}$\n",
    "   4. $f(x) = \\frac{x^2}{2x^2+3x+1}$\n",
    "   5. $f(x) = \\frac{1}{2x^2+3x+1}$\n",
    "   \n",
    "2. This question focuses on properties of the denominator $q(x)$.\n",
    "   1. Verify that if $f(x) = p(x)/q(x)$ and $q(x) = (x-r_1)(x-r_2) \\cdots (x-r_k)$ where the $r_k$ are all different from one another, then one of the $r_k=0$ if and only if $q(0)=0$.\n",
    "   2. Assume that $f(x) = p(x)/q(x)$ where $q(x) = C(x-r_1)(x-r_2) \\cdots (x-r_k)$ for some $C\\neq 0$, $C\\neq 1$.  Explain how we can rescale $p$ and $q$ so that $f(x) = \\hat{p}(x)/\\hat{q}(x)$ with $\\hat{q}(x) = (x-r_1)(x-r_2) \\cdots (x-r_k)$.\n"
   ]
  }
 ],
 "metadata": {
  "language_info": {
   "name": "python"
  }
 },
 "nbformat": 4,
 "nbformat_minor": 5
}