{
 "cells": [
  {
   "cell_type": "markdown",
   "id": "13ab03bd",
   "metadata": {},
   "source": [
    "(sec:GenFxnsDiff)=\n",
    "# Differentiation of Generating Functions\n",
    "\n",
    "A common operation that we will do with generating functions is to take their derivative.  If we have a generating function\n",
    "\n",
    "$$\n",
    "f(x) = c_0 + c_1 x + c_2 x^2 + \\cdots = \\sum_{n=0}^\\infty c_n x^n\n",
    "$$\n",
    "then \n",
    "\n",
    "$$\n",
    "f'(x) = c_1 + 2c_2 x + 3c_3 x^2 + \\cdots = \\sum_{n=0}^\\infty (n+1) c_{n+1} x^n\n",
    "$$\n",
    "So differentiating corresponds to multiplying the coefficient of $x^n$ by $n$ and reducing the power of $x$ by $1$.  In terms of the corresponding sequence of numbers, we multiply the $n$th number by $n$ and shift the indices so that it becomes the $n-1$st number.\n",
    "\n",
    "```{prf:example} Differentiation of a Poisson distribution PGF\n",
    ":label: example-DiffPoissonClothesLine\n",
    "\n",
    "Consider the PGF of a Poisson distribution with mean $2$:\n",
    "\n",
    "$$\n",
    "\\mu(x) = \\sum_{n=0}^\\infty \\frac{2^n e^{-2}}{n!} x^n\n",
    "$$\n",
    "\n",
    "If we differentiate this with respect to $x$ we get\n",
    "\n",
    "\\begin{align*}\n",
    "\\mu'(x) &= \\frac{d}{dx} \\sum_{n=0}^\\infty \\sum_{n=0}^\\infty n \\frac{2^n e^{-2}}{n!} x^{n}\\\\\n",
    "&= \\sum_{n=0}^\\infty n \\frac{2^n e^{-2}}{n!} x^{n-1}\\\\\n",
    "&= \\sum_{n=0}^\\infty (n+1) \\frac{2^{n+1}e^{-2}}{(n+1)!} x^n\n",
    "\\end{align*}\n",
    "where the final line reindexes the sum, eliminating the initial $0$ term.  This is illustrated in {numref}`fig-DiffPoissonClothesLine`.\n",
    "```\n",
    " \n",
    "\n",
    "```{figure} DiffPoissonClothesLine.png\n",
    "---\n",
    "width: 600px\n",
    "name: fig-DiffPoissonClothesLine\n",
    "\n",
    "---\n",
    "\n",
    "The \"clothesline\" (*i.e.*, series) representation of the PGF of the Poisson distribution with mean $2$ and its derivative.\n",
    "```\n",
    "\n",
    "If we don't want to shift the indices, that is, we want to keep the same power of $x$ we need to undo the reduction in power of $x$.  To do this, we multiply by $x$.\n",
    "\n",
    "$$\n",
    "x f'(x) = 0c_0 + 1 c_1 x + 2 c_2 x^2 + \\cdots= \\sum_{n=0}^\\infty n c_n x^n \n",
    "$$\n",
    "\n",
    "\n",
    "```{prf:example} Differentiation of a Poisson distribution PGF\n",
    ":label: example-xddxPoissonClothesLine\n",
    "\n",
    "If we start with the derivative of the PGF of a Poisson distribution with mean $2$:\n",
    "\n",
    "$$\n",
    "\\mu'(x) = \\sum_{n=0}^\\infty (n+1)\\frac{2^{n+1} e^{-2}}{(n+1)!} x^n\n",
    "$$\n",
    "and multiply by $x$ we get\n",
    "\n",
    "\\begin{align*}\n",
    "\\mu'(x)&= x\\sum_{n=0}^\\infty (n+1) \\frac{2^{n+1}e^{-2}}{(n+1)!} x^n\\\\\n",
    "&=\\sum_{n=0}^\\infty (n+1) \\frac{2^{n+1}e^{-2}}{(n+1)!} x^{n+1}\\\\\n",
    " &= \\sum_{n=0}^\\infty n \\frac{2^n e^{-2}}{n!} x^{n}\n",
    "\\end{align*}\n",
    "where the final line reindexes the sum, eliminating the initial $0$ term.  This is shown in {numref}`fig-xddxPoissonClothesLine`.  The result is \n",
    "```\n",
    "\n",
    "\n",
    "```{figure} xddxPoissonClothesLine.png\n",
    "---\n",
    "width: 600px\n",
    "name: fig-xddxPoissonClothesLine\n",
    "\n",
    "---\n",
    "\n",
    "The \"clothesline\" (*i.e.*, series) representation showing the multiplication of $\\mu'(x)$ by $x$.\n",
    "```\n",
    "\n",
    "\n",
    "\n",
    "So differentiating a generating function and then multiplying it by $x$ is equivalent to multiplying each $n$th term of the sequence by $n$.  Although we can do this with a series expansion, the benefit of this typically comes from when we have a closed form version of the function.  \n",
    "\n",
    "\n",
    "\n",
    "We will do this often.  For notational compactness we will use $x \\partial_x$ to denote taking the $x$ derivative and then multiplying the result by $x$:\n",
    "\n",
    "$$\n",
    "x \\partial_x f(x) = x f'(x) = \\sum n c_n x^n\n",
    "$$\n",
    "\n",
    "```{prf:example} $x \\partial_x$ of the Poisson Distribution PGF\n",
    ":label: example-xddxPoissonBag\n",
    "\n",
    "Consider the PGF of the Poisson Distribution of mean 2:\n",
    "\n",
    "\\begin{align*}\n",
    "\\mu(x) &= \\sum_{n=0}^\\infty \\frac{2^n e^{-2}}{n!}x^n\\\\\n",
    "&= e^{-2} \\sum_{n=0}^\\infty \\frac{(2x)^n}{n!}\\\\\n",
    "&= e^{-2}e^{2x}\\\\\n",
    "&= e^{2(x-1)}\n",
    "\\end{align*}\n",
    "When we take $x \\partial_x \\mu(x)$, we get\n",
    "\n",
    "\\begin{align*}\n",
    "x \\partial_x \\mu_x &= x \\frac{d}{dx} e^{2(x-1)}\\\\\n",
    "&= x (2e^{2(x-1)})\\\\\n",
    "&= 2x e^{2x-1}\n",
    "\\end{align*}\n",
    "This is illustrated in figure {numref}`fig-xddxPoissonBag`.\n",
    "```\n",
    "\n",
    "```{figure} xddxPoissonBag.png\n",
    "---\n",
    "width: 400px\n",
    "name: fig-xddxPoissonBag\n",
    "\n",
    "---\n",
    "\n",
    "Illustration of $x \\partial_x$ for the PGF of the Poisson distribution of mean $2$, using the \"bag\" representation.\n",
    "```\n",
    "\n",
    "When we perform the operation repeatedly, we will use the notation $(x \\partial_x)^k$:\n",
    "\n",
    "$$\n",
    "(x \\partial_x)^k f(x) = x \\partial_x (x \\partial_x)^{k-1} f(x) = \\sum n^k c_n x^n \n",
    "$$\n",
    "\n",
    "\n",
    "\n",
    "```{prf:example} The sequence $0^k, 1^k, 2^k, \\ldots$\n",
    "\n",
    "Consider the generating function\n",
    "\n",
    "$$\n",
    "A_k(x)= \\sum_{n=0}^\\infty n^k x^n = 0^k + 1^k x + 2^k x^2 + 3^k x^3 + \\cdots\n",
    "$$\n",
    "where $0^0$ is understood to be $1$.\n",
    "\n",
    "We have previously seen that\n",
    "\n",
    "$$\n",
    "A_0(x) = \\sum_{n=0}^\\infty 1 x^n = \\frac{1}{1-x}\n",
    "$$ \n",
    "To find $A_1(x) = \\sum_{n=0}^\\infty n x^n$ which corresponds to multiplying the $n$th term of the series in $A_0(x)$ by $n$, we simply differentiate $A_0(x)$ and multiply by $x$:\n",
    "\n",
    "\\begin{align*}\n",
    "A_1(x) &= \\sum_{n=0}^\\infty nx^n\\\\\n",
    "&= x \\partial_x A_0(x)\\\\\n",
    "&= x \\partial_x (1-x)^{-1}\\\\\n",
    "&= x(1-x)^{-2}\n",
    "\\end{align*}\n",
    "\n",
    "To find each successive $A_k(x)$ we repeat this with $A_k(x) = x \\partial_x A_{k-1}(x) = (x \\partial_x)^k \\frac{1}{1-x}$.\n",
    "```\n"
   ]
  },
  {
   "cell_type": "markdown",
   "id": "ac920e8c",
   "metadata": {},
   "source": [
    "```{prf:example} Calculating a Combinatorial Identity\n",
    ":label: example-CombIdent \n",
    "\n",
    "Consider the question:\n",
    "*What is the sum $\\sum_{n=0}^N n^2 \\binom{N}{n}$.*\n",
    "\n",
    "To find this sum, we will actually recast this as a special case of the more general question: *What is the sum $\\sum_{n=0}^N (xn)^2 \\binom{N}{n}$*.\n",
    "\n",
    "When $x=1$, this reduces to the original equation.  \n",
    "\n",
    "We observe that\n",
    "\n",
    "\\begin{align*}\n",
    "\\sum_{n=0}^N (xn)^2 \\binom{N}{n} &= \\sum_{n=0}^N n^2 \\binom{N}{n} x^n\\\\\n",
    "&= (x \\partial_x)^2 \\sum_{n=0}^N \\binom{N}{n} x^n\\\\\n",
    "&= (x \\partial_x)^2 (1+x)^N\\\\\n",
    "&= x \\partial_x \\left(x N(1+x)^{N-1}\\right)\\\\\n",
    "&= x \\left( N(1+x)^{N-1} + N(N-1)(1+x)^{N-2}\\right)\\\\\n",
    "&= Nx(1+x)^{N-1} + N(N-1) x(1+x)^{N-2}\n",
    "\\end{align*}\n",
    "The original question corresponded to $x=1$, so we substitute $x=1$ and get\n",
    "\n",
    "$$\\sum_{n=0}^N n^2 \\binom{N}{n} = 2^{N-1} N + 2^{N-2}N(N-1)$$\n",
    "```"
   ]
  },
  {
   "cell_type": "markdown",
   "id": "e3522c31",
   "metadata": {},
   "source": [
    "## Probability Generating Function applications\n",
    "\n",
    "\n",
    "In probability generating functions, the derivative has an important role to play.  \n",
    "\n",
    "### Moments of a distribution\n",
    "For a given distribution of the integers, we are often interested in the *moments* of the distribution, defined so that the $r$th moment is\n",
    "\n",
    "$$\\langle D^r \\rangle = \\mathbb{E}[D^r] = \\sum_{n=0}^\\infty n^r p_n\n",
    "$$\n",
    "\n",
    "If we take $\\mu(x) = \\sum p_n x^n$ to be the PGF of this distribution, then \n",
    "\\begin{align*}\n",
    "\\langle D \\rangle &= \\mathbb{E}[D^1] =\\sum_{n=0}^\\infty n p_n= \\sum_{n=0}^\\infty n p_n 1^n\\\\\n",
    "&  = \\left[ x \\partial_x \\mu(x) \\right|_{x=1}\\\\\n",
    "\\langle D^2 \\rangle  &= \\mathbb{E}[D^2] = \\sum_{n=0}^\\infty n^2 p_n= \\sum_{n=0}^\\infty n^2 p_n 1^n \\\\\n",
    "&= \\left[ (x \\partial_x)^2 \\mu(x) \\right|_{x=1}\n",
    "\\end{align*}\n",
    "and in general:\n",
    "\n",
    "\\begin{align*}\n",
    "\\langle D^r \\rangle &= \\mathbb{E}[D^r] =\\sum_{n=0}^\\infty n^r p_n= \\sum_{n=0}^\\infty n^r p_n 1^n \\\\\n",
    "&= \\left[ (x \\partial_x)^r \\mu(x)\\right|_{x=1}\n",
    "\\end{align*}\n",
    "\n",
    "Notice that $\\langle D^0 \\rangle = \\sum_{n=0}^\\infty p_n 1^n = 1$.  So $\\mu(1)=1$ if $\\mu(x)$ is a PGF.\n",
    "\n",
    "### Factorial Moments\n",
    "Sometimes we are interested in the *factorial moments*:\n",
    "\n",
    "$$\n",
    "\\langle (D)_r\\rangle = \\mathbb{E}[D(D-1)\\cdots(D-r+1) ] = \\sum_{n=0}^\\infty n(n-1)\\cdots (n-r+1) p_n\n",
    "$$\n",
    "In this case\n",
    "\\begin{align*}\n",
    "\\langle (D)_1 \\rangle &= \\mathbb{E}[D] =\\sum_{n=0}^\\infty n p_n= \\sum_{n=0}^\\infty n p_n 1^{n-1} \\\\\n",
    "& = \\mu'(1)\\\\\n",
    "\\langle (D)_2 \\rangle  &= \\mathbb{E}[D(D-1)] = \\sum_{n=0}^\\infty n(n-1) p_n= \\sum_{n=0}^\\infty n(n-1) p_n 1^{n-2} \\\\\n",
    "&= \\mu''(1)\n",
    "\\end{align*}\n",
    "and in general:\n",
    "\n",
    "\\begin{align*}\n",
    "\\langle (D)_r \\rangle &= \\mathbb{E}[D(D-1) \\cdot (D-r+1)] =\\sum_{n=0}^\\infty n(n-1)\\cdots (n-r+1) p_n= \\sum_{n=0}^\\infty n(n-1)\\cdots(n-r+1) p_n 1^{n-r} \\\\\n",
    "&= \\mu^{(r)}(1)\n",
    "\\end{align*}\n"
   ]
  },
  {
   "cell_type": "markdown",
   "id": "0b53ba4a",
   "metadata": {},
   "source": [
    "## Self-test\n",
    "\n",
    "1. Using the PGFs of the Binomial, Geometric, and Poisson distributions, find the average of each distribution in terms of the parameters appearing in the PGFs.\n",
    "\n",
    "2. Find the sum $\\sum_{n=0}^N n \\binom{N}{n}$.\n",
    "\n",
    "3. Find the sum $\\sum_{j=0}^\\infty j r^j$ for $|r|<1$.\n",
    "\n",
    "4. Consider a weighted coin that comes up heads with probability $p$ and tails with probability $1-p$.  Use differentiation of PGFs to find out how many flips on average it takes until the first heads (counting the final heads as a flip).\n",
    "   1. Explain why the probability of $n$ flips is $p(1-p)^{n-1}$, so the average is $p\\sum n (1-p)^{n-1}$.\n",
    "   2. Write this in terms of $\\mu'(1-p)$ for some PGF $\\mu(x)$ and find $\\mu(x)$.\n",
    "   3. Calculate the sum.\n",
    "\n",
    "\n"
   ]
  }
 ],
 "metadata": {
  "kernelspec": {
   "display_name": "Python 3",
   "language": "python",
   "name": "python3"
  },
  "language_info": {
   "codemirror_mode": {
    "name": "ipython",
    "version": 3
   },
   "file_extension": ".py",
   "mimetype": "text/x-python",
   "name": "python",
   "nbconvert_exporter": "python",
   "pygments_lexer": "ipython3",
   "version": "3.13.2"
  }
 },
 "nbformat": 4,
 "nbformat_minor": 5
}